examples/CIterationExamples/barthe.dfy
@@ -40,3 +40,19 @@ function f_loop1(n: int, c: int, i: int, j: int, x: int): int
   else
     x // The loop condition (i < n) failed; return x
 }
+
+lemma equivalenceHelper(n: int, c: int, i: int, j: int, x: int)
+  requires j == 5 * i + c
+  ensures f_loopM(n, c, i, j, x) == f_loop1(n, c, i, j, x)
+  decreases n - i
+{
+  if i < n {
+    equivalenceHelper(n, c, i + 1, j + 5, x + j);
+  }
+}
+
+lemma equivalence(n: int, c: int)
+  ensures fM(n, c) == f1(n, c)
+{
+  equivalenceHelper(n, c, 0, c, 0);
+}
